Reworking effects

src/coq/ReasoningFramework/OptimisationEffects.v
@@ -290,4 +290,482 @@ Qed.
 
 
 
+
+
+(* New *)
+
+Lemma trace_equiv_refl : reflexive (Trace ()) trace_equiv.
+Proof.
+  pcofix CIH. intro d.
+  pfold. destruct d; eauto.
+  - destruct v; eauto. destruct e; econstructor; eauto; constructor; apply related_effect_refl;
+    apply upaco2_refl; auto.
+Qed.
+
+Lemma trace_equiv_symm : symmetric (Trace ()) trace_equiv.
+Proof.
+  pcofix CIH.
+  intros d1 d2 H.
+  punfold H. 
+  induction H; pfold; econstructor; eauto.
+  - dependent destruction HRe; subst; eauto.
+    constructor. inversion HRe; constructor; eauto.
+    + intros. specialize (HRk a2 a1 (sym_eq H1)). pclearbot. right. eauto.
+    + intros. specialize (HRk v2 v1 (sym_eq H1)). pclearbot. right. eauto.
+    + pclearbot. right.  eauto.
+    + intros. specialize (HRk rv2 rv1 (sym_eq H1)). pclearbot. right. eauto.
+  - pclearbot. right. eauto.
+  - punfold IHtrace_equiv_step.
+  - punfold IHtrace_equiv_step.
+Qed.
+      
+
+Inductive tau_star (P:Trace () -> Prop) : Trace () -> Prop :=
+| tau_star_zero : forall (d:Trace ()), P d -> tau_star P d
+| tau_star_tau  : forall (d:Trace ()), tau_star P d -> tau_star P (Tau () d)
+.                                                       
+Hint Constructors tau_star.
+
+Lemma tau_star_monotone : monotone1 tau_star.
+Proof.
+  unfold monotone1.
+  intros x0 r r' IN LE.
+  induction IN; auto.
+Qed.  
+Hint Resolve tau_star_monotone : paco.
+
+(* This predicate relates two traces that agree on a non-tau step *)
+Inductive trace_event (R: Trace nat -> Trace nat -> Prop) : Trace nat -> Trace nat -> Prop :=
+| trace_event_vis : forall e1 e2, related_event_step R e1 e2 -> trace_event R (Vis e1) (Vis e2)
+.                                                                  
+Hint Constructors trace_event.
+
+Lemma trace_event_monotone : monotone2 trace_event.
+Proof.
+  unfold monotone2.
+  intros x0 x1 r r' IN LE.
+  induction IN; auto. constructor. eapply related_event_step_monotone; eauto.
+Qed.
+
+(*
+Inductive trace_equiv_big_step (R:Trace() -> Trace() -> Prop) : Trace() -> Trace() -> Prop :=
+| trace_equiv_big_diverge s1 s2 (DS1:diverges s1) (DS2:diverges s2) : trace_equiv_big_step R s1 s2
+| trace_equiv_big_taus s1 s2 t1 t2
+                     (TS1:tau_star (fun t => t = t1) s1)
+                     (TS2:tau_star (fun t => t = t2) s2)
+                     (HO: trace_event R t1 t2) : trace_equiv_big_step R s1 s2
+.                                                                 
+Hint Constructors trace_equiv_big_step.
+
+Lemma trace_equiv_big_step_monotone : monotone2 trace_equiv_big_step.
+Proof.
+  unfold monotone2.
+  intros x0 x1 r r' IN LE.
+  induction IN; auto.
+  eapply trace_equiv_big_taus. apply TS1. apply TS2.
+  eapply trace_event_monotone. apply HO. exact LE.
+Qed.  
+Hint Resolve trace_equiv_big_step_monotone : paco.
+
+Definition trace_equiv_big (d1 d2:Trace) := paco2 trace_equiv_big_step bot2 d1 d2.
+Hint Unfold trace_equiv_big.
+
+*)
+
+Lemma trace_equiv_tau_lft : forall (d1 d2:Trace ()), trace_equiv d1 d2 -> trace_equiv (Tau () d1) d2.
+Proof.
+  intros.
+  pfold. apply trace_equiv_step_lft.
+  punfold H.
+Qed.  
+
+Lemma trace_equiv_tau_rgt : forall (d1 d2:Trace ()), trace_equiv d1 d2 -> trace_equiv d1 (Tau () d2).
+Proof.
+  intros.
+  pfold. apply trace_equiv_step_rgt.
+  punfold H.
+Qed.  
+
+(*
+Lemma trace_equiv_lft_inversion : forall(d1 d2:Trace ()), trace_equiv (Tau () d1) d2 -> trace_equiv d1 d2.
+Proof.
+  intros d1 d2 H.
+  punfold H. remember (Tau d1) as d. 
+  induction H; try (solve [inversion Heqd; subst; clear Heqd]).
+  - inversion Heqd. subst. apply trace_equiv_tau_rgt. pclearbot. punfold HRk.
+  - inversion Heqd. subst. pfold. exact H.
+  - subst. apply trace_equiv_tau_rgt. apply IHtrace_equiv_step. reflexivity.
+Qed.    
+*)
+
+(*
+Lemma trace_equiv_rgt_inversion : forall (d1 d2:Trace ()), trace_equiv d1 (Tau () d2) -> trace_equiv d1 d2.
+Proof.
+  intros.
+  apply trace_equiv_symm. apply trace_equiv_symm in H. apply trace_equiv_lft_inversion. exact H.
+Qed.  
+*)
+
+(*
+Lemma event_not_diverges : forall (d:Trace), tau_star non_tau d -> diverges d -> False.
+Proof.
+  intros d HS.
+  induction HS.
+  - intros HD; dependent destruction d; punfold HD; inversion HD.
+  - intros HD. apply IHHS. punfold HD. dependent destruction HD. pclearbot. apply H.
+Qed.   
+*)
+
+ 
+(*
+(* CLASSICAL! *)
+Lemma event_or_diverges : forall (d:Trace), tau_star non_tau d \/ diverges d.
+Proof.
+  intros d.
+  destruct (classic (tau_star non_tau d)); eauto.
+  right. revert d H.
+  pcofix CIH.
+  intros d H.
+  destruct d; try solve [exfalso; apply H; constructor; simpl; auto].
+  pfold. econstructor. right. eauto.
+Qed.*)
+
+(*
+
+Lemma trace_equiv_diverges : forall (d1 d2:Trace) (EQ: trace_equiv d1 d2) (HD:diverges d1), diverges d2.
+Proof.
+  pcofix CIH.
+  intros d1 d2 EQ.
+  punfold EQ. induction EQ; intros HD; try solve [punfold HD; inversion HD].
+  - punfold HD. inversion HD. pclearbot. subst.
+    pfold. constructor. right. eauto.
+  - punfold HD. inversion HD. subst. pclearbot. apply IHEQ. apply H0.
+  - pfold. constructor. left. auto.
+Qed.    
+*)
+
+(*
+Lemma trace_equiv_event : forall (d1 d2:Trace) (EQ:trace_equiv d1 d2) (HS:tau_star non_tau d1), tau_star non_tau d2.
+Proof.
+  intros d1 d2 EQ HS.
+  revert d2 EQ.
+  induction HS; intros d2 EQ.
+  - punfold EQ. induction EQ; auto.
+    inversion H.
+  - punfold EQ. dependent induction EQ.
+    + apply tau_star_tau. apply IHHS. pclearbot. eauto.
+    + apply IHHS. pfold. exact EQ.
+    + apply tau_star_tau. eauto.
+Qed.      
+*)
+(*
+Lemma trace_equiv_diverges_or_event : forall (d1 d2:Trace ()) (EQ:trace_equiv d1 d2),
+    (diverges d1 /\ diverges d2) \/ (tau_star non_tau d1 /\ tau_star non_tau d2).
+Proof.
+  intros d1 d2 EQ.
+  destruct (@event_or_diverges d1) as [HS | HD].
+  - right. eauto using trace_equiv_event.
+  - left. eauto using trace_equiv_diverges.
+Qed.    
+*)
+
+
+(*
+Lemma trace_equiv_big_step_tau_left :  forall R (d1 d2:Trace)
+                                       (HR: paco2 trace_equiv_big_step R d1 d2), paco2 trace_equiv_big_step R (Tau d1) d2.
+Proof.
+  intros R d1 d2 HR.
+  punfold HR.
+  pfold.
+  destruct HR.
+  - apply trace_equiv_big_diverge; eauto. pfold. constructor. left. eauto.
+  - eapply trace_equiv_big_taus; eauto.
+Qed.
+*)
+
+
+(*
+Lemma trace_equiv_big_step_tau_right :  forall R (d1 d2:Trace)
+                                       (HR: paco2 trace_equiv_big_step R d1 d2), paco2 trace_equiv_big_step R d1 (Tau d2).
+Proof.
+  intros R d1 d2 HR.
+  punfold HR.
+  pfold.
+  destruct HR.
+  - apply trace_equiv_big_diverge; eauto. pfold. constructor. left. eauto.
+  - eapply trace_equiv_big_taus; eauto.
+Qed.
+*)
+
+
+(*
+Lemma trace_equiv_implies_trace_equiv_big: forall (d1 d2:Trace) (EQ:trace_equiv d1 d2), trace_equiv_big d1 d2.
+Proof.
+  pcofix CIH.
+  intros d1 d2 EQ.
+  destruct (@trace_equiv_diverges_or_event d1 d2 EQ) as [[HD1 HD2]|[HS1 HS2]]; eauto.
+  induction HS1.
+  - induction HS2.
+    + pfold. eapply trace_equiv_big_taus; try solve [eauto].
+      punfold EQ. dependent destruction EQ; eauto; try solve [simpl in H; inversion H]; try solve [simpl in H0; inversion H0].
+      constructor.
+      apply related_event_step_monotone with (R1 := (upaco2 trace_equiv_step bot2)).
+      intros d1 d2 H2. right.  eapply CIH. pclearbot. eapply H2.
+      exact HRe.
+    + eauto using trace_equiv_big_step_tau_right, trace_equiv_rgt_inversion.
+  - eauto using trace_equiv_big_step_tau_left, trace_equiv_lft_inversion.
+Qed.*)
+
+
+      (*
+Lemma trace_equiv_big_implies_trace_equiv : forall (d1 d2:Trace) (EQB:trace_equiv_big d1 d2), trace_equiv d1 d2.
+Proof.
+  pcofix CIH.
+  intros d1 d2 EQB.
+  punfold EQB. dependent destruction EQB.
+  - punfold DS1. punfold DS2.
+    dependent destruction DS1. dependent destruction DS2.
+    pfold. econstructor; eauto. right. apply CIH. pclearbot.
+    pfold. eapply trace_equiv_big_diverge; eauto.
+  - dependent induction TS1; subst.
+    + dependent induction TS2; subst.
+      * pfold. dependent destruction HO; eauto.
+        constructor. eapply related_event_step_monotone with (R1 := (upaco2 trace_equiv_big_step bot2)).
+        intros. right. apply CIH. pclearbot. eauto.
+        exact H.
+      * pfold.  apply IHTS2 in HO. punfold HO.
+    + pfold. constructor. apply IHTS1 in TS2; eauto. punfold TS2.
+Qed.      *)
+
+(*
+Lemma trace_event_non_tau_left : forall R (d1 d2:Trace), trace_event R d1 d2 -> non_tau d1.
+Proof.
+  intros R d1 d2 H.
+  dependent destruction H; simpl; auto.
+Qed.
+
+Lemma trace_event_non_tau_right : forall R (d1 d2:Trace), trace_event R d1 d2 -> non_tau d2.
+Proof.
+  intros R d1 d2 H.
+  dependent destruction H; simpl; auto.
+Qed.
+
+Lemma tau_star_non_tau_unique : forall (d d1 d2:Trace)
+   (TS1:tau_star (fun s => s = d1) d)
+   (TS2:tau_star (fun s => s = d2) d)
+   (NT1:non_tau d1)
+   (NT2:non_tau d2),
+    d1 = d2.
+Proof.
+  intros d d1 d2 TS1.
+  revert d2.
+  induction TS1; intros d2 TS2 ND1 ND2.
+  - induction TS2; subst; eauto.
+    + simpl in ND1. inversion ND1.
+  - dependent destruction TS2; eauto.
+    simpl in ND2. inversion ND2.
+Qed.    
+*)
+(*
+Lemma trace_equiv_mem_step_trans:
+  forall {A} (R : relation (Trace A)) (TR:transitive _ R) m1 m2 m3,
+    trace_equiv_mem_step R m1 m2 -> trace_equiv_mem_step R m2 m3 ->
+    trace_equiv_mem_step R m1 m3.
+Proof.
+  intros A R TR m1 m2 m3 H12 H23.
+  inversion H12; subst; inversion H23; subst; constructor; intros; eauto.
+Qed.
+ *)
+(*
+Lemma trace_equiv_mem_step_trans:
+  forall {A} (m1 m2 m3:effects A),
+    trace_equiv_mem_step m1 m2 -> trace_equiv_mem_step m2 m3 ->
+    trace_equiv_mem_step m1 m3.
+Proof.
+  intros A m1 m2 m3 H12 H23.
+  inversion H12; subst; inversion H23; subst; constructor; intros; eauto.
+  - rewrite H. rewrite H3. reflexivity.
+  - rewrite H. rewrite H3. reflexivity.
+  - rewrite H. rewrite H4. reflexivity.    
+Qed.
+*)
+(*
+Lemma trace_equiv_big_trans : forall (d1 d2 d3:Trace), trace_equiv_big d1 d2 -> trace_equiv_big d2 d3 -> trace_equiv_big d1 d3.
+Proof.
+  pcofix CIH.
+  intros d1 d2 d3 EQB1 EQB2.
+  punfold EQB1. punfold EQB2.
+  destruct EQB1, EQB2; eauto.
+  - exfalso. eapply event_not_diverges, DS2.
+    eapply tau_star_monotone. apply TS1.
+    intros s PR. simpl in PR.  subst. eauto using trace_event_non_tau_left.
+  - exfalso. eapply event_not_diverges, DS1.
+    eapply tau_star_monotone. apply TS2.
+    intros s PR. simpl in PR. subst. eauto using trace_event_non_tau_right.
+  - eapply tau_star_non_tau_unique in TS2; eauto using trace_event_non_tau_left, trace_event_non_tau_right.
+    subst.
+    pfold. eapply trace_equiv_big_taus; eauto.
+    destruct HO; dependent destruction HO0; eauto.
+    econstructor.
+    dependent destruction H; dependent destruction H0; constructor; eauto.
+    dependent destruction HRe; dependent destruction HRe0; constructor; eauto.
+    + intros a1 a2 Heq.
+      specialize (HRk a1 a2 Heq). specialize (HRk0 a1 a2 Heq). subst. pclearbot.
+      right. eapply CIH; eauto.
+    + intros v1 v2 Heq.
+      specialize (HRk v1 v2 Heq). specialize (HRk0 v1 v2 Heq). subst. pclearbot.
+      right. eapply CIH; eauto.
+    + pclearbot. right. eapply CIH; eauto.
+    + intros rv1 rv2 Heq.
+      specialize (HRk rv1 rv2 Heq). specialize (HRk0 rv1 rv2 Heq). subst. pclearbot.
+      right. eapply CIH; eauto.
+Qed.    
+    
+*)
+
+(*
+Lemma trace_equiv_trans : forall (d1 d2 d3:Trace ()), trace_equiv d1 d2 -> trace_equiv d2 d3 -> trace_equiv d1 d3.
+Proof.
+  eauto using trace_equiv_big_trans, trace_equiv_implies_trace_equiv_big, trace_equiv_big_implies_trace_equiv.
+Qed.
+*)
+
+
+
+(* This statement is false if d1 and d2 are inifinite Tau streams
+    would have to weaken the conclusion to:
+      (d1 = d2 /\ d1 = all_taus) \/ ... 
+    this would probably require classical logic to prove.
+
+Lemma trace_equiv_inversion : forall {A} (d1 d2:Trace A),
+    trace_equiv d1 d2 ->  exists d1', exists d2', exists n, exists m,
+            d1 = taus n d1' /\ d2 = taus m d2' /\ non_tau_head d1' /\ non_tau_head d2' /\ trace_equiv d1' d2'.
+Proof.
+Abort.  
+*)
+
+
+(* stuttering --------------------------------------------------------------- *)
+
+
+
+
+Fixpoint taus (n:nat) (d:Trace ()) : Trace () :=
+  match n with
+  | 0 => d
+  | S n => Tau () (taus n d)
+  end.
+
+(*
+Lemma stutter_simpl : forall (d1 d2: Trace ()) n, trace_equiv (taus n d1) d2 -> trace_equiv d1 d2.
+Proof.
+  intros. induction n. punfold H.
+  eapply IHn. simpl in H. eapply trace_equiv_lft_inversion. eapply H.
+Qed.
+*)
+
+(*
+Lemma stutter : forall (d1 d2: Trace ()) n m, trace_equiv (taus n d1) (taus m d2) -> trace_equiv d1 d2.
+Proof.
+  intros.
+  eapply stutter_simpl.
+  eapply trace_equiv_symm.
+  eapply stutter_simpl.
+  eapply trace_equiv_symm.
+  eauto.
+Qed.
+*)
+
+
+(* error-free traceervations -------------------------------------------------- *)
+
+
+Section PREDICATE_EFFECTS.
+  Variable X : Type.
+  Variable R : X -> Prop.
+
+  Inductive predicate_effect_step  : effects X -> Prop :=
+  | predicate_effect_Alloca :
+      forall t k
+        (HRk : forall (a:addr), R (k (inj_addr a))),
+        predicate_effect_step (Alloca t k)
+
+  | predicate_effect_Load :
+      forall a k
+        (HRk : forall (v:value), R (k v)),
+        predicate_effect_step (Load a k)
+
+  | predicate_effect_Store  :
+      forall a v k
+        (HRk : R (k no_value)),
+        predicate_effect_step (Store a v k)
+
+  | predicate_effect_Call :
+      forall v vs k
+        (HRk : forall (rv:value), R (k rv)),
+        predicate_effect_step (Call v vs k)
+  .
+End PREDICATE_EFFECTS.
+
+Hint Constructors predicate_effect_step.
+
+
+Lemma predicate_effect_step_monotone : forall X (R1 R2: X -> Prop)
+                                        (HR: forall d, R1 d -> R2 d) e
+                                        (HM:predicate_effect_step R1 e),
+    predicate_effect_step R2 e.
+Proof.
+  intros X R1 R2 HR e HM.
+  dependent destruction HM; constructor; eauto.
+Qed.  
+Hint Resolve predicate_effect_step_monotone : paco.
+
+
+Inductive error_free_event_step {X} (R : X -> Prop) : Event X -> Prop :=
+| error_free_event_fin :
+    forall v,
+      error_free_event_step R (Fin v)
+
+| error_free_event_eff :
+      forall e
+        (HRe : predicate_effect_step R e),
+        error_free_event_step R (Eff e)
+.
+Hint Constructors error_free_event_step.
+
+Lemma error_free_event_step_monotone : forall X (R1 R2: X -> Prop)
+                                        (HR: forall d, R1 d -> R2 d) e
+                                        (HM:error_free_event_step R1 e),
+    error_free_event_step R2 e.
+Proof.
+  intros X R1 R2 HR e HM.
+  dependent destruction HM; constructor; eauto.
+  eapply predicate_effect_step_monotone; eauto.
+Qed.  
+Hint Resolve error_free_event_step_monotone : paco.
+
+Inductive error_free_trace_step (R : Trace() -> Prop) : Trace() -> Prop :=
+| error_free_vis : forall e, error_free_event_step R e -> error_free_trace_step R (Vis e)
+| error_free_tau : forall k, R k -> error_free_trace_step R (Tau () k)
+.                                                  
+Hint Constructors error_free_trace_step.
+
+Lemma error_free_trace_step_monotone : monotone1 error_free_trace_step.
+Proof.
+  unfold monotone1.
+  intros x0 r r' IN LE.
+  induction IN; constructor; eauto.
+  eapply error_free_event_step_monotone; eauto.
+Qed.
+Hint Resolve error_free_trace_step_monotone : paco.
+
+Definition error_free_trace d := paco1 error_free_trace_step bot1 d.
+Hint Unfold error_free_trace.
+
 End Effects.
+
+
+
+
+
+
